Wrote some laws for sets. Tried to solve exercise 2.1 from Okasaki, but failed.

Basic/BinomialTree.v
@@ -191,10 +191,98 @@ Proof.
           apply inj_pair2 in H4. inv H3.
   destruct f as [| r t f'].
     right. inv 1.
-    destruct (elem_dec A x (S r) t).
-      left. auto.
+    destruct (elem_dec A x _ t).
+      left. constructor. auto.
       destruct (elemForest_dec A x _ f').
         left. auto.
         right. inv 1; apply inj_pair2 in H1; apply inj_pair2 in H3;
           subst; inv H2.
 Defined.
+
+End wut3.
+
+Module wut4.
+
+Inductive BinomialTree (A : Type) : nat -> Type :=
+    | node : A -> forall {r : nat}, BinomialForest A r -> BinomialTree A r
+
+with BinomialForest (A : Type) : nat -> Type :=
+    | bfnil : BinomialForest A 0
+    | bfcons : forall {r : nat},
+        BinomialTree A r -> BinomialForest A r ->
+          BinomialForest A (S r).
+
+Arguments node {A} _ {r} _.
+Arguments bfnil {A}.
+Arguments bfcons {A r} _ _.
+
+Inductive elem {A : Type} (x : A)
+  : forall {r : nat}, BinomialTree A r -> Prop :=
+    | elemC :
+        forall (y : A) (r : nat) (f : BinomialForest A r),
+          x = y \/ elemForest x f -> elem x (node y f)
+
+with elemForest {A : Type} (x : A)
+  : forall {r : nat}, BinomialForest A r -> Prop :=
+    | elemForestC :
+        forall (r : nat) (t : BinomialTree A r) (f : BinomialForest A r),
+          elem x t \/ elemForest x f -> elemForest x (bfcons t f).
+
+Hint Constructors elem elemForest.
+
+Fixpoint elem_dec
+  {A : LinDec} (x : A) {r : nat} (t : BinomialTree A r) :
+    {elem x t} + {~ elem x t}
+
+with elemForest_dec
+  {A : LinDec} (x : A) {r : nat} (f : BinomialForest A r) :
+    {elemForest x f} + {~ elemForest x f}.
+Proof.
+  destruct t as [y r f].
+    case_eq (x =? y); intros.
+      left. dec.
+      destruct (elemForest_dec A x _ f).
+        left. auto.
+        right. inv 1.
+          dec.
+          apply inj_pair2 in H4. inv H3.
+  destruct f as [| r t f'].
+    right. inv 1.
+    destruct (elem_dec A x _ t).
+      left. constructor. auto.
+      destruct (elemForest_dec A x _ f').
+        left. auto.
+        right. inv 1; apply inj_pair2 in H1; apply inj_pair2 in H3;
+          subst; inv H2.
+Defined.
+
+Definition BinomialHeap (A : Type) : Type :=
+  {r : nat & list (BinomialTree A r)}.
+
+Print BinomialTree.
+
+Definition link {A : LinDec} {r : nat} (t1 t2 : BinomialTree A r)
+  : BinomialTree A (S r).
+Proof.
+  destruct t1 as [x r ts], t2 as [x' r ts'].
+    destruct (x <=? x').
+      exact (node x (bfcons (node x' ts') ts)).
+      exact (node x' (bfcons (node x ts) ts')). Show Proof.
+Defined.
+Restart.
+  refine (
+match t1 in (BinomialTree _ r)
+         return (BinomialTree A r -> BinomialTree A (S r))
+with
+    | @node _ x r ts =>
+        fun t2 =>
+        match t2 in (BinomialTree _ r)
+                 return (BinomialForest A r -> BinomialTree A (S r))
+        with
+            | @node _ x' r ts' =>
+                fun ts : BinomialForest A r =>
+                if x <=? x'
+                then node x (bfcons (node x' ts') ts)
+                else node x' (bfcons (node x ts) ts')
+        end ts
+end t2).
