ADT/Set.v
@@ -14,13 +14,45 @@ Parameter empty :
 Parameter isEmpty :
   forall {A : LinDec}, S A -> bool.
 
-Parameter put :
+(** TODO: rename [put]. *)
+Parameter insert :
   forall {A : LinDec}, A -> S A -> S A.
 
-Parameter del :
+(** TODO: rename [del]. *)
+Parameter remove :
   forall {A : LinDec}, A -> S A -> S A.
 
-Parameter has :
+(** TODO: rename [has]. *)
+Parameter member :
   forall {A : LinDec}, A -> S A -> bool.
+
+(** Properties of [member]. *)
+
+Parameter member_insert :
+  forall (A : LinDec) (x : A) (s : S A),
+    member x (insert x s) = true.
+
+Parameter member_insert' :
+  forall (A : LinDec) (x y : A) (s : S A),
+    member x (insert y s) =
+    if x =? y then true else member x s.
+
+Parameter member_remove :
+  forall (A : LinDec) (x : A) (s : S A),
+    member x (remove x s) = false.
+
+Parameter member_remove' :
+  forall (A : LinDec) (x y : A) (s : S A),
+    member x (remove y s) =
+    if x =? y then false else member x s.
+
+(** Definition of equivalent sets. *)
+
+Definition equiv {A : LinDec} (s1 s2 : S A) : Prop :=
+  forall x : A, member x s1 = member x s2.
+
+Parameter remove_insert_equiv :
+  forall (A : LinDec) (x : A) (s : S A),
+    equiv (remove x (insert x s)) s.
 
 End SET.
